Conform/TestRunner.lean
@@ -1,5 +1,7 @@
 import EvmYul.EVM.State
 import EvmYul.EVM.Semantics
+import EvmYul.EVM.Gas
+import EvmYul.Wheels
 
 import EvmYul.State.TransactionOps
 import EvmYul.State.Withdrawal
@@ -108,18 +110,6 @@ end
 def executeTransaction (transaction : Transaction) (s : EVM.State) (header : BlockHeader) : Except EVM.Exception EVM.State := do
   let _TODOfuel := 2^13
 
-  -- Validate transaction
-  match transaction with
-    | .blob t =>
-      if t.maxFeePerBlobGas.toNat < header.getBlobGasprice then .error (.TransactionException .INSUFFICIENT_MAX_FEE_PER_BLOB_GAS)
-      if header.blobGasUsed == none || header.excessBlobGas == none then .error (.TransactionException .TYPE_3_TX_PRE_FORK)
-      match t.blobVersionedHashes with
-        | [] => .error (.TransactionException .TYPE_3_TX_ZERO_BLOBS)
-        | hs =>
-          if hs.any (λ h ↦ h[0]? != .some VERSIONED_HASH_VERSION_KZG) then
-            .error (.TransactionException .TYPE_3_TX_ZERO_BLOBS)
-    | _ => pure ()
-
   let (ypState, substate, z) ← EVM.Υ (debugMode := false) _TODOfuel s.accountMap header.chainId.toNat header.baseFeePerGas header s.genesisBlockHeader s.blocks transaction transaction.base.expectedSender
 
   -- as EIP 4788 (https://eips.ethereum.org/EIPS/eip-4788).
@@ -133,125 +123,301 @@ def executeTransaction (transaction : Transaction) (s : EVM.State) (header : Blo
   }
   pure result
 
+
+def validateTransaction
+  (σ : AccountMap)
+  (chainId : ℕ)
+  (header : BlockHeader)
+  (expectedSender : AccountAddress)
+  (T : Transaction)
+  : Except EVM.Exception Unit
+:= do
+  if T.base.nonce.toNat ≥ 2^64-1 then
+    .error <| .TransactionException .NONCE_IS_MAX
+
+  let g₀ : ℕ := EVM.intrinsicGas T
+  if T.base.gasLimit.toNat < g₀ then
+    .error <| .TransactionException .INTRINSIC_GAS_TOO_LOW
+
+  match T with
+    | .blob t =>
+      if t.maxFeePerBlobGas.toNat < header.getBlobGasprice then .error (.TransactionException .INSUFFICIENT_MAX_FEE_PER_BLOB_GAS)
+      match t.blobVersionedHashes with
+        | [] => .error (.TransactionException .TYPE_3_TX_ZERO_BLOBS)
+        | hs =>
+          if hs.any (λ h ↦ h[0]? != .some VERSIONED_HASH_VERSION_KZG) then
+            .error (.TransactionException .TYPE_3_TX_ZERO_BLOBS)
+    | .dynamic t =>
+      if t.maxPriorityFeePerGas > t.maxFeePerGas then .error <| .TransactionException .InconsistentFees
+    | _ => pure ()
+
+  match T.base.recipient with
+    | none => do
+      let MAX_CODE_SIZE := 24576
+      let MAX_INITCODE_SIZE := 2 * MAX_CODE_SIZE
+      if T.base.data.size > MAX_INITCODE_SIZE then
+        .error <| .TransactionException .INITCODE_SIZE_EXCEEDED
+    | some _ => pure ()
+
+  let H_f := header.baseFeePerGas
+  let some T_RLP := RLP (← (L_X T)) | .error <| .TransactionException .IllFormedRLP
+
+  -- let g₀ : ℕ := EVM.intrinsicGas T
+
+  -- if T.base.gasLimit.toNat < g₀ then
+  --   .error <| .TransactionException .INTRINSIC_GAS_TOO_LOW
+
+  let r : ℕ := fromBytesBigEndian T.base.r.data.data
+  let s : ℕ := fromBytesBigEndian T.base.s.data.data
+  if 0 ≥ r ∨ r ≥ secp256k1n then .error <| .TransactionException .InvalidSignature
+  if 0 ≥ s ∨ s > secp256k1n / 2 then .error <| .TransactionException .InvalidSignature
+  let v : ℕ := -- (324)
+    match T with
+      | .legacy t =>
+        let w := t.w.toNat
+        if w ∈ [27, 28] then
+          w - 27
+        else
+          if w = 35 + chainId * 2 ∨ w = 36 + chainId * 2 then
+            (w - 35) % 2 -- `chainId` not subtracted in the Yellow paper but in the EEL spec
+          else
+            w
+      | .access t | .dynamic t | .blob t => t.yParity.toNat
+  if v ∉ [0, 1] then .error <| .TransactionException .InvalidSignature
+
+  let h_T := -- (318)
+    match T with
+      | .legacy _ => KEC T_RLP
+      | _ => KEC <| ByteArray.mk #[T.type] ++ T_RLP
+
+  let (S_T : AccountAddress) ← -- (323)
+    match ECDSARECOVER h_T (ByteArray.mk #[.ofNat v]) T.base.r T.base.s with
+      | .ok s =>
+        pure <| Fin.ofNat <| fromBytesBigEndian <|
+          ((KEC s).extract 12 32 /- 160 bits = 20 bytes -/ ).data.data
+      | .error s => .error <| .SenderRecoverError s
+  if S_T != expectedSender then
+    dbg_trace s!"Recovered sender ({EvmYul.toHex S_T.toByteArray}) ≠ expected sender ({EvmYul.toHex expectedSender.toByteArray})"
+  -- dbg_trace s!"Looking for S_T: {S_T} in: σ: {repr σ}"
+
+  -- "Also, with a slight abuse of notation ... "
+  let (senderCode, senderNonce, senderBalance) :=
+    match σ.find? S_T with
+      | some sender => (sender.code, sender.nonce, sender.balance)
+      | none =>
+        dbg_trace s!"could not find sender {EvmYul.toHex S_T.toByteArray}"
+        (.empty, ⟨0⟩, ⟨0⟩)
+
+
+  if senderCode ≠ .empty then .error <| .TransactionException .SENDER_NOT_EOA
+  if T.base.nonce < senderNonce  then .error <| .TransactionException .NONCE_MISMATCH_TOO_LOW
+  if T.base.nonce > senderNonce then .error <| .TransactionException .NONCE_MISMATCH_TOO_HIGH
+  let v₀ :=
+    match T with
+      | .legacy t | .access t => t.gasLimit * t.gasPrice + t.value
+      | .dynamic t => t.gasLimit * t.maxFeePerGas + t.value
+      | .blob t    => t.gasLimit * t.maxFeePerGas + t.value + (UInt256.ofNat <| (getTotalBlobGas T).getD 0) * t.maxFeePerBlobGas
+  -- dbg_trace s!"v₀: {v₀}, senderBalance: {senderBalance}"
+  if v₀ > senderBalance then .error <| .TransactionException .INSUFFICIENT_ACCOUNT_FUNDS
+
+  if H_f >
+    match T with
+      | .dynamic t | .blob t => t.maxFeePerGas.toNat
+      | .legacy t | .access t => t.gasPrice.toNat
+  then .error <| .TransactionException .BaseFeeTooHigh
+
+  let n :=
+    match T.base.recipient with
+      | some _ => T.base.data.size
+      | none => 0
+  if n > 49152 then .error <| .TransactionException .INITCODE_SIZE_EXCEEDED
+
+ where
+  L_X (T : Transaction) : Except EVM.Exception 𝕋 := -- (317)
+    let accessEntryRLP : AccountAddress × Array UInt256 → 𝕋
+      | ⟨a, s⟩ => .𝕃 [.𝔹 (AccountAddress.toByteArray a), .𝕃 (s.map (𝕋.𝔹 ∘ UInt256.toByteArray)).toList]
+    let accessEntriesRLP (aEs : List (AccountAddress × Array UInt256)) : 𝕋 :=
+      .𝕃 (aEs.map accessEntryRLP)
+    match T with
+      | /- 0 -/ .legacy t =>
+        if t.w.toNat ∈ [27, 28] then
+          .ok ∘ .𝕃 ∘ List.map .𝔹 <|
+            [ BE t.nonce.toNat -- Tₙ
+            , BE t.gasPrice.toNat -- Tₚ
+            , BE t.gasLimit.toNat -- T_g
+            , -- If Tₜ is ∅ it becomes the RLP empty byte sequence and thus the member of 𝔹₀
+              t.recipient.option .empty AccountAddress.toByteArray -- Tₜ
+            , BE t.value.toNat -- Tᵥ
+            , t.data
+            ]
+        else
+          if t.w = .ofNat (35 + chainId * 2) ∨ t.w = .ofNat (36 + chainId * 2) then
+            .ok ∘ .𝕃 ∘ List.map .𝔹 <|
+              [ BE t.nonce.toNat -- Tₙ
+              , BE t.gasPrice.toNat -- Tₚ
+              , BE t.gasLimit.toNat -- T_g
+              , -- If Tₜ is ∅ it becomes the RLP empty byte sequence and thus the member of 𝔹₀
+                t.recipient.option .empty AccountAddress.toByteArray -- Tₜ
+              , BE t.value.toNat -- Tᵥ
+              , t.data -- p
+              , BE chainId
+              , .empty
+              , .empty
+              ]
+          else
+            dbg_trace "IllFormedRLP legacy transacion: Tw = {t.w}; chainId = {chainId}"
+            .error <| .TransactionException .IllFormedRLP
+
+      | /- 1 -/ .access t =>
+        .ok ∘ .𝕃 <|
+          [ .𝔹 (BE t.chainId.toNat) -- T_c
+          , .𝔹 (BE t.nonce.toNat) -- Tₙ
+          , .𝔹 (BE t.gasPrice.toNat) -- Tₚ
+          , .𝔹 (BE t.gasLimit.toNat) -- T_g
+          , -- If Tₜ is ∅ it becomes the RLP empty byte sequence and thus the member of 𝔹₀
+            .𝔹 (t.recipient.option .empty AccountAddress.toByteArray) -- Tₜ
+          , .𝔹 (BE t.value.toNat) -- T_v
+          , .𝔹 t.data  -- p
+          , accessEntriesRLP <| Batteries.RBSet.toList t.accessList -- T_A
+          ]
+      | /- 2 -/ .dynamic t =>
+        .ok ∘ .𝕃 <|
+          [ .𝔹 (BE t.chainId.toNat) -- T_c
+          , .𝔹 (BE t.nonce.toNat) -- Tₙ
+          , .𝔹 (BE t.maxPriorityFeePerGas.toNat) -- T_f
+          , .𝔹 (BE t.maxFeePerGas.toNat) -- Tₘ
+          , .𝔹 (BE t.gasLimit.toNat) -- T_g
+          , -- If Tₜ is ∅ it becomes the RLP empty byte sequence and thus the member of 𝔹₀
+            .𝔹 (t.recipient.option .empty AccountAddress.toByteArray) -- Tₜ
+          , .𝔹 (BE t.value.toNat) -- Tᵥ
+          , .𝔹 t.data -- p
+          , accessEntriesRLP <| Batteries.RBSet.toList t.accessList -- T_A
+          ]
+      | /- 3 -/ .blob t =>
+        .ok ∘ .𝕃 <|
+          [ .𝔹 (BE t.chainId.toNat) -- T_c
+          , .𝔹 (BE t.nonce.toNat) -- Tₙ
+          , .𝔹 (BE t.maxPriorityFeePerGas.toNat) -- T_f
+          , .𝔹 (BE t.maxFeePerGas.toNat) -- Tₘ
+          , .𝔹 (BE t.gasLimit.toNat) -- T_g
+          , -- If Tₜ is ∅ it becomes the RLP empty byte sequence and thus the member of 𝔹₀
+            .𝔹 (t.recipient.option .empty AccountAddress.toByteArray) -- Tₜ
+          , .𝔹 (BE t.value.toNat) -- Tᵥ
+          , .𝔹 t.data -- p
+          , accessEntriesRLP <| Batteries.RBSet.toList t.accessList -- T_A
+          , .𝔹 (BE t.maxFeePerBlobGas.toNat)
+          , .𝕃 (t.blobVersionedHashes.map .𝔹)
+          ]
+
+def validateBlock (parentHeader : BlockHeader) (block : Block)
+  : Except EVM.Exception (Transactions × Withdrawals)
+:= do
+  -- dbg_trace "VALIDATING BLOCK"
+  if calcExcessBlobGas parentHeader != block.blockHeader.excessBlobGas then
+    throw <| .BlockException .INCORRECT_EXCESS_BLOB_GAS
+
+  match block.blockHeader.blobGasUsed, block.blockHeader.excessBlobGas with
+  | some _, none | none, some _ =>
+    throw <| .BlockException .INCORRECT_BLOCK_FORMAT
+  | _, _ => pure ()
+
+  let blobGasUsed := List.sum <| Array.data <| block.transactions.map ((Option.getD · 0) ∘  getTotalBlobGas)
+
+  match block.blockHeader.blobGasUsed with
+    | none => pure ()
+    | some bGU =>
+      if blobGasUsed != bGU.toNat then
+        throw <| .BlockException .INCORRECT_BLOB_GAS_USED
+
+  let MAX_BLOB_GAS_PER_BLOCK := 786432
+  if blobGasUsed > MAX_BLOB_GAS_PER_BLOCK then
+    throw <| .BlockException .BLOB_GAS_USED_ABOVE_LIMIT
+
+  if block.blockHeader.withdrawalsRoot.isSome && computeTrieRoot block.withdrawals ≠ block.blockHeader.withdrawalsRoot then
+    throw <| .BlockException .INVALID_WITHDRAWALS_ROOT
+
+  -- dbg_trace "BLOCK VALID"
+  pure (block.transactions, block.withdrawals)
 /--
 This assumes that the `transactions` are ordered, as they should be in the test suit.
 -/
 def processBlocks (s₀ : EVM.State) : Except EVM.Exception EVM.State := do
   let blocks := s₀.blocks
-
-  -- Validate `excessBlobGas`
   let parentHeaders := #[s₀.genesisBlockHeader] ++ blocks.map Block.blockHeader
   let withParentHeaders := parentHeaders.zip blocks
-  withParentHeaders.forM
-    λ (parentHeader, block) ↦ do
-      if calcExcessBlobGas parentHeader != block.blockHeader.excessBlobGas then
-        -- if !block.exception.isEmpty then
-        let e : EVM.Exception := .BlockException_INCORRECT_EXCESS_BLOB_GAS
-        if block.exception.containsSubstr (repr e).pretty then
-          dbg_trace s!"Expected exception: {block.exception}; got exception: {repr e}"
-          throw <| EVM.Exception.ExpectedException s₀.accountMap
-        else
-          throw <| .BlockException_INCORRECT_EXCESS_BLOB_GAS
 
-  blocks.foldlM processBlock s₀
-  where processBlock (s : EVM.State) (block : Block) : Except EVM.Exception EVM.State := do
-    -- We should not check the timestamp. Some tests have timestamp less than 1710338135 but still need EIP-4788
-    -- let FORK_TIMESTAMP := 1710338135
-    let _TODOfuel := 2^13
-    let SYSTEM_ADDRESS : AccountAddress := 0xfffffffffffffffffffffffffffffffffffffffe
-    let BEACON_ROOTS_ADDRESS : AccountAddress := 0x000F3df6D732807Ef1319fB7B8bB8522d0Beac02
-    let MAX_BLOB_GAS_PER_BLOCK := 786432
-
-    -- dbg_trace s!"blobGasUsed: {block.blockHeader.blobGasUsed}, excessBlobGas: {block.blockHeader.excessBlobGas}"
-    match block.blockHeader.blobGasUsed, block.blockHeader.excessBlobGas with
-      | some _, none | none, some _ =>
-        -- if !block.exception.isEmpty then
-        let e : EVM.Exception := .BlockException_INCORRECT_BLOCK_FORMAT
-        if block.exception.containsSubstr (repr e).pretty then
-          dbg_trace s!"Expected exception: {block.exception}; got exception: {repr e}"
-          throw <| EVM.Exception.ExpectedException s.accountMap
-        else
-          throw <| .BlockException_INCORRECT_BLOCK_FORMAT
-      | _, _ => pure ()
-
-    -- Validate `blobGasUsed`
-    let blobGasUsed := List.sum <| Array.data <| block.transactions.map ((Option.getD · 0) ∘  getTotalBlobGas)
-    match block.blockHeader.blobGasUsed with
-      | none => pure ()
-      | some bGU =>
-        if blobGasUsed != bGU.toNat || blobGasUsed > MAX_BLOB_GAS_PER_BLOCK then
-          -- if !block.exception.isEmpty then
-          let e : EVM.Exception := .BlockException_INCORRECT_BLOB_GAS_USED
+  withParentHeaders.foldlM processBlock s₀
+ where
+  processBlock (s₀ : EVM.State) (withParentHeader : BlockHeader × Block) : Except EVM.Exception EVM.State := do
+    let (parentHeader, block) := withParentHeader
+    let (encounteredBlockException, transactions, s, withdrawals) ←
+      match validateBlock parentHeader block with
+        | .error e =>
           if block.exception.containsSubstr (repr e).pretty then
             dbg_trace s!"Expected exception: {block.exception}; got exception: {repr e}"
-            throw <| EVM.Exception.ExpectedException s.accountMap
+            pure (true, #[], s₀, #[])
           else
-            throw <| .BlockException_INCORRECT_BLOB_GAS_USED
+            throw e
+        | .ok (ts, ws) =>
+          let BEACON_ROOTS_ADDRESS : AccountAddress := 0x000F3df6D732807Ef1319fB7B8bB8522d0Beac02
+          let SYSTEM_ADDRESS : AccountAddress := 0xfffffffffffffffffffffffffffffffffffffffe
+          let s ←
+          match s₀.accountMap.find? BEACON_ROOTS_ADDRESS with
+            | none => pure (false, ts, s₀, ws)
+            | some roots =>
+              let beaconRootsAddressCode := roots.code
+              let _TODOfuel := 2^13
+              -- the call does not count against the block’s gas limit
+              let (createdAccounts, σ, _, substate, _ /- can't fail-/, _) ←
+                EVM.Θ (debugMode := false) _TODOfuel
+                  []
+                  .empty
+                  s₀.genesisBlockHeader
+                  s₀.blocks
+                  s₀.accountMap
+                  default
+                  SYSTEM_ADDRESS
+                  SYSTEM_ADDRESS
+                  BEACON_ROOTS_ADDRESS
+                  (.Code beaconRootsAddressCode)
+                  ⟨30000000⟩
+                  ⟨0xe8d4a51000⟩
+                  ⟨0⟩
+                  ⟨0⟩
+                  block.blockHeader.parentBeaconBlockRoot
+                  0
+                  block.blockHeader
+                  true
+              let s :=
+                {s₀ with
+                  createdAccounts := createdAccounts
+                  accountMap := σ
+                  substate := substate
+                }
+              pure (false, ts, s, ws)
 
-    -- if no code exists at `BEACON_ROOTS_ADDRESS`, the call must fail silently
-    let s ←
-      match s.accountMap.find? BEACON_ROOTS_ADDRESS with
-        | none => pure s
-        | some roots =>
-          let beaconRootsAddressCode := roots.code
-          -- the call does not count against the block’s gas limit
-          let (createdAccounts, σ, _, substate, _ /- can't fail-/, _) ←
-            EVM.Θ
-              (debugMode := false)
-              _TODOfuel
-              []
-              .empty
-              s.genesisBlockHeader
-              s.blocks
-              s.accountMap
-              default
-              SYSTEM_ADDRESS
-              SYSTEM_ADDRESS
-              BEACON_ROOTS_ADDRESS
-              (.Code beaconRootsAddressCode)
-              ⟨30000000⟩
-              ⟨0xe8d4a51000⟩
-              ⟨0⟩
-              ⟨0⟩
-              block.blockHeader.parentBeaconBlockRoot
-              0
-              block.blockHeader
-              true
-          pure <|
-            {s with
-              createdAccounts := createdAccounts
-              accountMap := σ
-              substate := substate
-            }
     -- dbg_trace "\nStarting transactions"
-    let s ← block.transactions.foldlM
-      (λ s trans ↦
-        try
-          executeTransaction trans s block.blockHeader
-        catch e =>
-          if block.exception.containsSubstr (repr e).pretty then
-            dbg_trace s!"Expected exception: {block.exception}; got exception: {repr e}"
-            throw <| EVM.Exception.ExpectedException s.accountMap
-          else throw e
-      )
-      s
-    let σ ←
-      match block.blockHeader.withdrawalsRoot with
-        | some wR =>
-          ( try
-            applyWithdrawals
-              s.accountMap
-              wR
-              block.withdrawals
-            catch e =>
-              if block.exception.containsSubstr (repr e).pretty then
-                dbg_trace s!"Expected exception: {block.exception}; got exception: {repr e}"
-                throw <| EVM.Exception.ExpectedException s.accountMap
-              else throw e
-          )
-        | none => pure s.accountMap
-    pure <| { s with accountMap := σ }
-    -- pure s
+    let (encounteredTransactionException, s) ←
+      try
+        let s ←
+          transactions.foldlM
+            (λ s' trans ↦ do
+              validateTransaction s'.accountMap block.blockHeader.chainId.toNat block.blockHeader trans.base.expectedSender trans
+              executeTransaction trans s' block.blockHeader
+            )
+            s
+        let σ := applyWithdrawals s.accountMap withdrawals
+        pure <| (false, { s with accountMap := σ })
+      catch e =>
+        if block.exception.containsSubstr (repr e).pretty then
+          dbg_trace s!"Expected exception: {block.exception}; got exception: {repr e}"
+          pure (true, s₀)
+        else throw e
+
+    if ¬encounteredBlockException && ¬encounteredTransactionException && ¬block.exception.isEmpty then
+      throw <| .MissedExpectedException block.exception
+    pure s
+
 
 /--
 - `.none` on success
@@ -260,7 +426,6 @@ def processBlocks (s₀ : EVM.State) : Except EVM.Exception EVM.State := do
 NB we can throw away the final state if it coincided with the expected one, hence `.none`.
 -/
 def preImpliesPost (pre : Pre) (post : Post) (genesisBlockHeader : BlockHeader) (blocks : Blocks) : Except EVM.Exception (Option AccountMap) := do
-  try
     let resultState ← processBlocks {pre.toEVMState with blocks := blocks, genesisBlockHeader := genesisBlockHeader}
     let result : AddrMap AccountEntry :=
       resultState.toState.accountMap.foldl
@@ -270,17 +435,6 @@ def preImpliesPost (pre : Pre) (post : Post) (genesisBlockHeader : BlockHeader) 
         dbg_trace e
         pure (.some resultState.accountMap) -- Feel free to inspect this error from `almostBEqButNotQuite`.
       | .ok _ => pure .none
-  catch
-    | .ExpectedException σ =>
-      -- let result : AddrMap AccountEntry :=
-      --   σ.foldl
-      --     (λ r addr ⟨nonce, balance, storage, _, _, code⟩ ↦ r.insert addr ⟨nonce, balance, storage, code⟩) default
-      -- TODO: I think we should check the state after the last valid block, but now we just use the pre
-      if post == pre then
-        pure .none -- An expected exception was thrown, which means the test is ok.
-      else
-        pure (.some σ)
-    | e                    => throw e
 
 -- local instance : MonadLift (Except EVM.Exception) (Except Conform.Exception) := ⟨Except.mapError .EVMError⟩
 -- vvvvvvvvvvvvvv DO NOT DELETE PLEASE vvvvvvvvvvvvvvvvvv
