EvmYul/EVM/Exception.lean
@@ -17,100 +17,133 @@ inductive ExecutionException where
   -- | PRECOMPILE_FAILURE
   -- | NONCE_EXCEEDED
 
-inductive TransactionExceptionException where
-  | IllFormedRLP : TransactionExceptionException
-  | InvalidSignature : TransactionExceptionException
-  | InvalidSenderNonce : TransactionExceptionException
-  | SenderCodeNotEmpty : TransactionExceptionException
-  | INSUFFICIENT_ACCOUNT_FUNDS : TransactionExceptionException
-  | BaseFeeTooHigh : TransactionExceptionException
-  | InconsistentFees : TransactionExceptionException
-  | InitCodeDataGreaterThan49152 : TransactionExceptionException
-  | TYPE_3_TX_ZERO_BLOBS : TransactionExceptionException
-  | TYPE_3_TX_PRE_FORK : TransactionExceptionException
-  | INTRINSIC_GAS_TOO_LOW : TransactionExceptionException
-  | INSUFFICIENT_MAX_FEE_PER_BLOB_GAS : TransactionExceptionException
-  | INITCODE_SIZE_EXCEEDED : TransactionExceptionException
-  | MAX_CODE_SIZE_EXCEEDED : TransactionExceptionException
-  | NONCE_IS_MAX : TransactionExceptionException
+instance : Repr ExecutionException where
+  reprPrec s _ :=
+    match s with
+      | .OutOfFuel => "OutOfFuel"
+      | .InvalidInstruction => "InvalidInstruction"
+      | .OutOfGass => "OutOfGass"
+      | .BadJumpDestination => "BadJumpDestination"
+      | .StackOverflow => "StackOverflow"
+      | .StackUnderflow => "StackUnderflow"
+      | .InvalidMemoryAccess => "InvalidMemoryAccess"
+      | .StaticModeViolation => "StaticModeViolation"
 
-instance : Repr TransactionExceptionException where
+inductive BlockException where
+  | INCORRECT_EXCESS_BLOB_GAS
+  | INCORRECT_BLOB_GAS_USED
+  | INCORRECT_BLOCK_FORMAT -- TODO: No "Cancun" test needs this
+  | BLOB_GAS_USED_ABOVE_LIMIT
+  | INVALID_WITHDRAWALS_ROOT
+
+instance : Repr BlockException where
+  reprPrec s _ :=
+    match s with
+      | .INCORRECT_EXCESS_BLOB_GAS => "INCORRECT_EXCESS_BLOB_GAS"
+      | .INCORRECT_BLOB_GAS_USED => "INCORRECT_BLOB_GAS_USED"
+      | .INCORRECT_BLOCK_FORMAT => "INCORRECT_BLOCK_FORMAT"
+      | .BLOB_GAS_USED_ABOVE_LIMIT => "BLOB_GAS_USED_ABOVE_LIMIT"
+      | .INVALID_WITHDRAWALS_ROOT => "INVALID_WITHDRAWALS_ROOT"
+
+inductive TransactionException where
+  | IllFormedRLP
+  | InvalidSignature
+  | NONCE_MISMATCH_TOO_LOW
+  | NONCE_MISMATCH_TOO_HIGH
+  | SENDER_NOT_EOA
+  | INSUFFICIENT_ACCOUNT_FUNDS
+  | BaseFeeTooHigh
+  | InconsistentFees
+  | TYPE_3_TX_ZERO_BLOBS
+  | TYPE_3_TX_PRE_FORK -- TODO: No "Cancun" test needs this
+  | INTRINSIC_GAS_TOO_LOW
+  | INSUFFICIENT_MAX_FEE_PER_BLOB_GAS
+  | INITCODE_SIZE_EXCEEDED
+  | MAX_CODE_SIZE_EXCEEDED
+  | NONCE_IS_MAX
+  | TYPE_3_TX_BLOB_COUNT_EXCEEDED
+  | GAS_ALLOWANCE_EXCEEDED -- TODO: What is this
+
+instance : Repr TransactionException where
   reprPrec s _ :=
     match s with
       | .IllFormedRLP         => "IllFormedRLP"
       | .InvalidSignature     => "InvalidSignature"
-      | .InvalidSenderNonce   => "InvalidSenderNonce"
-      | .SenderCodeNotEmpty   => "SenderCodeNotEmpty"
+      | .NONCE_MISMATCH_TOO_LOW   => "NONCE_MISMATCH_TOO_LOW"
+      | .NONCE_MISMATCH_TOO_HIGH   => "NONCE_MISMATCH_TOO_HIGH"
+      | .SENDER_NOT_EOA   => "SENDER_NOT_EOA"
       | .INSUFFICIENT_ACCOUNT_FUNDS => "INSUFFICIENT_ACCOUNT_FUNDS"
       | .BaseFeeTooHigh       => "BaseFeeTooHigh"
       | .InconsistentFees     => "InconsistentFees"
-      | .InitCodeDataGreaterThan49152  => "InitCodeDataGreaterThan49152"
       | .TYPE_3_TX_ZERO_BLOBS => "TYPE_3_TX_ZERO_BLOBS"
       | .TYPE_3_TX_PRE_FORK => "TYPE_3_TX_PRE_FORK"
       | .INTRINSIC_GAS_TOO_LOW => "INTRINSIC_GAS_TOO_LOW"
-      | .INSUFFICIENT_MAX_FEE_PER_BLOB_GAS => "INTRINSIC_GAS_TOO_LOW"
+      | .INSUFFICIENT_MAX_FEE_PER_BLOB_GAS => "INSUFFICIENT_MAX_FEE_PER_BLOB_GAS"
       | .INITCODE_SIZE_EXCEEDED => "INITCODE_SIZE_EXCEEDED"
       | .MAX_CODE_SIZE_EXCEEDED => "MAX_CODE_SIZE_EXCEEDED"
       | .NONCE_IS_MAX => "NONCE_IS_MAX"
+      | .TYPE_3_TX_BLOB_COUNT_EXCEEDED => "TYPE_3_TX_BLOB_COUNT_EXCEEDED"
+      | .GAS_ALLOWANCE_EXCEEDED => "GAS_ALLOWANCE_EXCEEDED"
 
 -- TODO - fix / cleanup.
 inductive Exception where
-  | StackUnderflow                            : Exception
-  | StackOverflow                             : Exception
-  | BadJumpDestination                          : Exception
-  | InvalidMemoryAccess                         : Exception
-  | StaticModeViolation                         : Exception
-  | InvalidPC                                   : Exception
-  | OutOfBounds                                 : Exception
-  | NotEncodableRLP                             : Exception
-  | InvalidInstruction                          : Exception
-  | SenderMustExist                             : Exception
-  | ReceiverMustExistWithNonZeroValue           : Exception
-  | Underflow                                   : Exception
-  | Overflow                                    : Exception
+  -- | OutOfFuel :                                   Exception
+  -- | InvalidInstruction :                          Exception
+  -- | OutOfGass :                                   Exception
+  -- | BadJumpDestination :                          Exception
+  -- | StackOverflow :                               Exception
+  -- | StackUnderflow :                              Exception
+  -- | InvalidMemoryAccess :                         Exception
+  -- | StaticModeViolation :                         Exception
+  | ExecutionException :     ExecutionException → Exception
+  -- | InvalidPC                                   : Exception
+  -- | OutOfBounds                                 : Exception
+  | NotEncodableRLP :                             Exception
+  -- | SenderMustExist                             : Exception
+  -- | ReceiverMustExistWithNonZeroValue           : Exception
+  -- | Underflow                                   : Exception
+  -- | Overflow                                    : Exception
   -- | StopInvoked (s : EVM.State)                 : Exception
-  | OutOfFuel                                   : Exception
-  | OutOfGass                                   : Exception
-  | TransactionException :
-                    TransactionExceptionException → Exception
-  | ReceiverNotInAccounts (a : AccountAddress)  : Exception
-  | InvalidWithdrawal (s : String) : Exception
-  | BogusExceptionToBeReplaced (s : String) : Exception
-  | ExpectedException (post : AccountMap)   : Exception
-  | SenderRecoverError             : String → Exception
-  | BlockException_INCORRECT_EXCESS_BLOB_GAS : Exception
-  | BlockException_INCORRECT_BLOB_GAS_USED : Exception
-  | BlockException_INCORRECT_BLOCK_FORMAT
+  | TransactionException : TransactionException → Exception
+  -- | ReceiverNotInAccounts (a : AccountAddress)  : Exception
+  -- | InvalidWithdrawal (s : String) : Exception
+  -- | BogusExceptionToBeReplaced (s : String) : Exception
+  -- | ExpectedException (post : AccountMap)   : Exception
+  | SenderRecoverError :                 String → Exception
+  | BlockException :             BlockException → Exception
+  | MissedExpectedException :            String → Exception
 
 instance : Repr Exception where
   reprPrec s _ :=
     match s with
-      | .StaticModeViolation => "StaticModeViolation"
-      | .BadJumpDestination                => "BadJumpDestination"
-      | .InvalidMemoryAccess               => "InvalidMemoryAccess"
-      | .StackUnderflow                    => "StackUnderflow"
-      | .StackOverflow                     => "StackOverflow"
-      | .InvalidPC                         => "InvalidPC"
-      | .OutOfBounds                       => "OutOfBounds"
-      | .NotEncodableRLP                   => "NotEncodableRLP"
-      | .InvalidInstruction                => "InvalidInstruction"
-      | .SenderMustExist                   => "SenderMustExist"
-      | .ReceiverMustExistWithNonZeroValue => "ReceiverMustExistWithNonZeroValue"
-      | .Underflow                         => "Underflow"
-      | .Overflow                          => "Overflow"
+      | .ExecutionException ee =>       "Execution exception: " ++ repr ee
+      -- | .StaticModeViolation =>         "StaticModeViolation"
+      -- | .BadJumpDestination =>          "BadJumpDestination"
+      -- | .InvalidMemoryAccess =>         "InvalidMemoryAccess"
+      -- | .StackUnderflow =>              "StackUnderflow"
+      -- | .StackOverflow =>               "StackOverflow"
+      -- | .InvalidPC                         => "InvalidPC"
+      -- | .OutOfBounds                       => "OutOfBounds"
+      | .NotEncodableRLP =>             "NotEncodableRLP"
+      -- | .InvalidInstruction =>          "InvalidInstruction"
+      -- | .SenderMustExist                   => "SenderMustExist"
+      -- | .ReceiverMustExistWithNonZeroValue => "ReceiverMustExistWithNonZeroValue"
+      -- | .Underflow                         => "Underflow"
+      -- | .Overflow                          => "Overflow"
       -- | .StopInvoked _                     => "Execution halted by STOP."
-      | .OutOfFuel                         => "OutOfFuel"
-      | .OutOfGass                         => "OutOfGass"
-      | .TransactionException e              => "TransactionException." ++ repr e
-      | .ReceiverNotInAccounts
-          (a : AccountAddress)             => s!"ReceiverNotInAccounts: {a}"
-      | .InvalidWithdrawal s               => s!"InvalidWithdrawal: {s}"
-      | .BogusExceptionToBeReplaced s      => s!"BogusExceptionToBeReplaced: {s}"
-      | .ExpectedException _               => s!"Expected exception"
-      | .SenderRecoverError s              => "SenderRecoverError." ++ s
-      | .BlockException_INCORRECT_EXCESS_BLOB_GAS => "BlockException.INCORRECT_EXCESS_BLOB_GAS"
-      | .BlockException_INCORRECT_BLOB_GAS_USED => "BlockException.INCORRECT_BLOB_GAS_USED"
-      | .BlockException_INCORRECT_BLOCK_FORMAT => "BlockException.INCORRECT_BLOCK_FORMAT"
+      -- | .OutOfFuel =>                   "OutOfFuel"
+      -- | .OutOfGass =>                   "OutOfGass"
+      | .TransactionException e =>      "TransactionException." ++ repr e
+      -- | .ReceiverNotInAccounts
+      --     (a : AccountAddress)             => s!"ReceiverNotInAccounts: {a}"
+      -- | .InvalidWithdrawal s               => s!"InvalidWithdrawal: {s}"
+      -- | .BogusExceptionToBeReplaced s      => s!"BogusExceptionToBeReplaced: {s}"
+      -- | .ExpectedException _               => s!"Expected exception"
+      | .SenderRecoverError s =>        "SenderRecoverError." ++ s
+      | .BlockException be =>           "BlockException." ++ repr be
+      | .MissedExpectedException mee => "Missed expected exception" ++ mee
+
+#eval repr (Exception.BlockException .INCORRECT_EXCESS_BLOB_GAS)
 
 end EVM
 
